

$$
\mathcal{L}[f(t)] = \int_0^\infty f(t)e^{-st} \, dt
$$

$$
\mathcal{L}[1] = \frac{1}{s}
$$

$$
\mathcal{L}[n] = \frac{n}{s}
$$

$$
\mathcal{L}[e^{at}] = \frac{1}{s-a}
$$

$$
\mathcal{L}\left[6 - 5e^t + 3e^{2t}\right] = \frac{6}{s} - \frac{5}{s-4} + \frac{3}{s-2}
$$

$$
\mathcal{L}[\sinh at] =  \frac{e^{at} - e^{-at}}{2} = \frac{1}{2}\left(\frac{1}{s-a} - \frac{1}{s+a}\right) = \frac{a}{s^2 - a^2}
$$







$$
\cosh x = \frac{e^x + e^{-x}}{2}
$$

$$
\cosh at = \frac{e^{at} + e^{-at}}{2}
$$

$$
\mathcal{L}[\cosh at] = \frac{s}{s^2 - a^2}
$$

$$
\mathcal{L}[\sinh 5t] = \frac{5}{s^2 - 25}
$$




-----

**Lunes 27:** Cuaderno  
**Martes 28:** Examen



$$
\mathcal{L}[\sinh at] = \frac{a}{s^2 - a^2}
$$

$$
\mathcal{L}[\cosh at] = \frac{s}{s^2 - a^2}
$$



